examples/low-level/crypto/Crypto.Symmetric.MAC.fst
@@ -36,55 +36,68 @@ let elem i = (* dependent; used only ideally *)
 (** Private representation of a field element as a buffer *)
 
 (* 16-10-26 for the time being, we avoid value-dependent types (after
-   erasure and flag inlining) for kremlin. We may later compile those
-   two untagged unions. We also use a top-level refinement, so that
+   erasure and flag inlining) for Kremlin. We may later compile those
+   to untagged unions. We also use a top-level refinement, so that
    case analysis applies without pattern matching.
    
    See 35380a8a for an older, more type-dependent version *)
 
-unfold inline_for_extraction let limb = function
+unfold inline_for_extraction 
+let limb = function
   | POLY1305 -> UInt64.t
   | GHASH    -> UInt8.t
-let limb_length = function 
+
+unfold inline_for_extraction
+let limb_length = function
   | POLY1305 ->  5
   | GHASH    -> 16
 
-unfold inline_for_extraction type buffer' a = b:Buffer.buffer (limb a){Buffer.length b == limb_length a} 
-noeq type buffer'' =
-  | B_POLY1305 of buffer' POLY1305
-  | B_GHASH    of buffer' GHASH
-abstract type elemB i = b:buffer''
-  { match alg i with 
-  | POLY1305 -> is_B_POLY1305 b 
+inline_for_extraction
+type buffer_of a = b:Buffer.buffer (limb a){Buffer.length b == limb_length a}
+
+// private?
+noeq type _buffer =
+  | B_POLY1305 of buffer_of POLY1305
+  | B_GHASH    of buffer_of GHASH
+
+abstract type elemB i = b:_buffer
+  { match alg i with
+  | POLY1305 -> is_B_POLY1305 b
   | GHASH    -> is_B_GHASH b }
-let as_buffer (#i:id) (b:elemB i) : GTot(buffer' (alg i)) =
-  match b with
+
+val as_buffer: #i:id -> elemB i -> GTot (buffer_of (alg i))
+let as_buffer #i = function
   | B_POLY1305 b -> b
   | B_GHASH    b -> b
- 
-let live h #i (b:elemB i) = Buffer.live h (as_buffer b)
-let norm h #i (b:elemB i) =
-  match b with
+
+val live: mem -> #i:id -> elemB i -> Type0
+let live h #i b = Buffer.live h (as_buffer b)
+
+val norm: mem -> #i:id -> b:elemB i -> Type0
+let norm h #i = function
   | B_POLY1305 b -> Crypto.Symmetric.Poly1305.Bigint.norm h b // implies live
   | B_GHASH    b -> Buffer.live h b
 
+
 (** message words (not necessarily a full word. *)
 let wlen = 16ul
+
 type word = b:Seq.seq u8{Seq.length b <= UInt32.v wlen}
+
 type word_16 = lbytes (UInt32.v wlen)
 
 (** Mutable representation of (partial) words as buffers *)
 type wordB = b:Buffer.buffer u8{Buffer.length b <= UInt32.v wlen}
+
 type wordB_16 = lbuffer (UInt32.v wlen)
 
-let sel_word (h:mem) (b:wordB{Buffer.live h b}) : GTot word =
-  Buffer.as_seq h b
+val sel_word: h:mem -> b:wordB{Buffer.live h b} -> GTot word
+let sel_word h b = Buffer.as_seq h b
 
 val sel_elem: h:mem -> #i:id -> b:elemB i{live h b} -> GTot (elem i)
-let sel_elem h #i b =
-  match b with
+let sel_elem h #i = function
   | B_POLY1305 b -> PL.sel_elem h b
-  | B_GHASH    b -> Buffer.as_seq #UInt8.t h b
+  | B_GHASH    b -> Buffer.as_seq h b
 
 (** Create and initialize an element (used for r) *)
 val rcreate: rgn:HH.rid{HS.is_eternal_region rgn} -> i:id -> ST (elemB i)
@@ -92,7 +105,6 @@ val rcreate: rgn:HH.rid{HS.is_eternal_region rgn} -> i:id -> ST (elemB i)
   (ensures  (fun h0 r h1 ->
     HS.modifies (Set.singleton rgn) h0 h1 /\
     HS.modifies_ref rgn TSet.empty h0 h1))
-
 let rcreate rgn i =
   match alg i with
   | POLY1305 -> B_POLY1305 (FStar.Buffer.rcreate rgn 0UL  5ul)
@@ -107,15 +119,21 @@ let create i =
   | POLY1305 -> B_POLY1305 (FStar.Buffer.create 0uL 5ul)
   | GHASH    -> B_GHASH    (FStar.Buffer.create 0uy 16ul)
 
-// TODO: generalize length, add functional spec & modifies clause
+// TODO: generalize length, add functional spec
 (** Encode raw bytes of static key as a field element *)
 val encode_r: #i:id -> b:elemB i -> raw:lbuffer 16{Buffer.disjoint (as_buffer b) raw} -> Stack unit
   (requires (fun h -> live h b /\ Buffer.live h raw))
-  (ensures  (fun h0 _ h1 -> live h1 b))
+  (ensures  (fun h0 _ h1 -> live h1 b /\ Buffer.live h1 raw 
+    /\ Buffer.modifies_2 (as_buffer b) raw h0 h1))
 let encode_r #i b raw =
   match b with 
   | B_POLY1305 b -> PL.clamp raw; PL.toField b raw
-  | B_GHASH    b -> Buffer.blit raw 0ul b 0ul 16ul
+  | B_GHASH    b -> 
+    begin
+    let h0 = ST.get () in
+    assert (Buffer.modifies_1 raw h0 h0); // Necessary for triggering right lemmas
+    Buffer.blit raw 0ul b 0ul 16ul
+    end
 
 // TODO: generalize to word
 (** Encode a word of a message as a field element *)
@@ -130,7 +148,7 @@ private val encodeB: i:id -> w:wordB_16 -> StackInline (elemB i)
   (requires (fun h -> Buffer.live h w))
   (ensures  (fun h0 b h1 -> Buffer.live h1 w /\ live h1 b /\ norm h1 b
     /\ Buffer.modifies_0 h0 h1
-    /\ ~(live h0 b)
+    /\ ~(Buffer.contains h0 (as_buffer b))
     /\ sel_elem h1 b == encode i (sel_word h1 w)))
 let encodeB i w =
   match alg i with 
@@ -170,26 +188,27 @@ val field_mul: #i:id -> elem i -> elem i -> Tot (elem i)
 let field_mul #i a b =
   match alg i with
   | POLY1305 -> PS.field_mul a b
-  | GHASH    -> GS.op_Plus_At a b
+  | GHASH    -> GS.op_Star_At a b
 
 let op_Plus_At #i e1 e2 = field_add #i e1 e2
 let op_Star_At #i e1 e2 = field_mul #i e1 e2
 
 #set-options "--z3timeout 20 --initial_fuel 0 --max_fuel 0"
 
+
 (** Process one message block and update the accumulator *)
 val update: #i:id -> r:elemB i -> a:elemB i -> w:wordB_16 -> Stack unit
   (requires (fun h -> live h r /\ live h a /\ Buffer.live h w
     /\ norm h r /\ norm h a
-    /\ Buffer.disjoint_2 (as_buffer r) (as_buffer a) w /\ Buffer.disjoint (as_buffer a) w))
+    /\ Buffer.disjoint_2 (as_buffer r) (as_buffer a) w 
+    /\ Buffer.disjoint (as_buffer a) w))
   (ensures  (fun h0 _ h1 ->
-    live h0 a /\ live h0 r /\ Buffer.live h0 w /\ live h1 a /\ live h1 r
+    live h0 a /\ live h0 r /\ Buffer.live h0 w /\ live h1 a ///\ live h1 r
     /\ norm h1 a
     /\ Buffer.modifies_1 (as_buffer a) h0 h1
-//    /\ sel_elem h1 a == (sel_elem h0 a +@ encode i (sel_word h0 w)) *@ sel_elem h0 r
-      ))
+    /\ sel_elem h1 a == (sel_elem h0 a +@ encode i (sel_word h0 w)) *@ sel_elem h0 r))
 
-#reset-options "--z3timeout 20"
+// TODO: use encodeB?
 let update #i r a w =
   let h0 = ST.get () in
   match r, a with
@@ -210,16 +229,15 @@ let update #i r a w =
       pop_frame();
 
       let h3 = ST.get () in
-      Crypto.Symmetric.Poly1305.Bigint.eval_eq_lemma h2 h3 a a 5;
-      assume false //16-10-26 
+      Crypto.Symmetric.Poly1305.Bigint.eval_eq_lemma h2 h3 a a 5
     end
-  | B_GHASH r, B_GHASH a ->
-    begin
-      GF.add_and_multiply a w r
-    end
+  | B_GHASH r, B_GHASH a -> GF.add_and_multiply a w r
+
 
 let taglen = 16ul
+
 type tag = lbytes (UInt32.v taglen) 
+
 type tagB = lbuffer (UInt32.v taglen)
 
 (** Complete MAC-computation specifications *)
@@ -235,22 +253,27 @@ val finish: #i:id -> s:tagB -> a:elemB i -> t:tagB -> Stack unit
     Buffer.live h s /\ 
     norm h a /\ 
     Buffer.live h t /\
-    Buffer.disjoint_2 (as_buffer a) s t /\ Buffer.disjoint s t ))
-  (ensures  (fun h0 () h1 -> 
-    Buffer.live h1 s /\
-    norm h1 a /\
-    Buffer.live h1 t /\
-    Buffer.modifies_2 (as_buffer a) t h0 h1 /\ (
-    let tv = Buffer.as_seq h1 t in 
-    let sv = Buffer.as_seq h1 s in 
-    let av = sel_elem h1 a in
-    match alg i with 
+    Buffer.disjoint_2 (as_buffer a) s t /\ Buffer.disjoint s t))
+  (ensures  (fun h0 _ h1 -> live h0 a /\ Buffer.live h0 s
+    /\ live h1 a
+    /\ Buffer.live h1 s
+    /\ Buffer.live h1 t
+    /\ Buffer.modifies_2 (as_buffer a) t h0 h1
+    /\ (
+    let tv = Buffer.as_seq h1 t in
+    let sv = Buffer.as_seq h0 s in
+    let av = sel_elem h0 a in
+    match alg i with
     | POLY1305 -> Seq.equal tv (PS.finish av sv)
     | GHASH    -> Seq.equal tv (GS.finish av sv) )))
 
-#reset-options "--lax" 
 let finish #i s a t =
-  match a with 
+  match a with
   | B_POLY1305 a -> PL.poly1305_finish t a s
-  | B_GHASH    a -> GF.finish a s; 
-                   Buffer.blit a 0ul t 0ul 16ul
+  | B_GHASH    a ->
+    begin
+    GF.finish a s;
+    Buffer.blit a 0ul t 0ul 16ul;
+    let h1 = ST.get() in
+    Seq.lemma_eq_intro (Buffer.as_seq h1 t) (Seq.slice (Buffer.as_seq h1 t) 0 16)
+    end
